%====
% Appendix B: 2 p2.p3
%====
\section{Evaluating $2 p_2 \cdot p_3$}
\newcommand{\Qvec}[1]{\bm{Q}_{#1}}
\newcommand{\Qmag}[1]{|\bm{Q}_{#1}|}
\label{app:2-dot-3}
Let $\varepsilon_i = Q_i^0 = \sqrt{\Qmag{i}^2 + t_i}$. Then,
\begin{equation}
    \begin{aligned}
        p_2 \cdot p_3 
        &=
            (Q_1 - Q_2)\cdot(Q_2 - Q_3)     \\
        &=
            Q_1 \cdot Q_2 - Q_1 \cdot Q_3 - t_2 + Q_2 \cdot Q_3 \\
        &= 
            \varepsilon_1 \varepsilon_2 - \Qvec{1}\cdot\Qvec{2}
        -
            \varepsilon_1 \varepsilon_3 - \Qvec{1}\cdot\Qvec{3}
        -
            t_2
        +
        \varepsilon_2 \varepsilon_3 - \Qvec{2}\cdot\Qvec{3} \, . 
    \end{aligned}
\end{equation}
To simplify things we choose to measure angles relative to $\Qvec{3} = -\bm{p}_b$. Therefore, 
\begin{align}
    \Qvec{1} &= \cos \varphi_1 \sin \theta_1 \hat{\bm{i}} + \sin \varphi_1 \sin \theta_1 \hat{\bm{j}} + \cos \theta_1 \hat{\bm{k}} \\
    \Qvec{2} &= \cos \varphi_2 \sin \theta_2 \hat{\bm{i}} + \sin \varphi_2 \sin \theta_2 \hat{\bm{j}} + \cos \theta_2 \hat{\bm{k}} \\
    \Qvec{3} &= \hat{\bm{k}} \; .
\end{align}
Thus,
\begin{align}
    p_2 \cdot p_3 
    =\  
        &\varepsilon_1 \varepsilon_2 - \Qmag{1}\Qmag{2} 
        \big[
            \sin \theta_1 \sin \theta_2 \cos(\varphi_1 - \varphi_2) + \cos\theta_1 \cos\theta_2
        \big]\\
    &-
        \varepsilon_1 \varepsilon_3 - \Qmag{1}\Qmag{3} \cos \theta_1
    -
        t_2
    +
    \varepsilon_2 \varepsilon_3 - \Qmag{2}\Qmag{3} \cos \theta_2 \; .
\end{align}
But, 
\begin{gather}
    \begin{aligned}
        \Qmag{i} &= \frac{\sqrt{\lambda(s_i, t_i, m_a^2)}}{2 m_a} \\
        \varepsilon_i &= \frac{t_i - s_i - m_a^2}{2 m_a} \\
        \cos \theta_i & = 
            \frac
                {
                    (t_i - s_i - m_a^2)(t_{i+1} - s_{i+1} - m_a^2) - 2m_a^2(t_i + t_{i+1} - m_n^2)
                }
                {
                    \sqrt{
                        \lambda(s_i, t_i, m_a^2) \lambda(s_{i+1},t_{i+1}, m_a^2)
                    }
                } \\
        \sin \theta^2_i & = 
                -
                \frac
                    {
                        m_a^2
                    }
                    {
                        \lambda(s_{i+1}, t_{i+1}, m_a^2) \lambda(s_i, t_i, m_a^2)
                    } \, 
                G(t_i, s_{i+1}, t_i, t_{i+1}, m_{i+1}^2, m_a^2) 
    \end{aligned}
\end{gather}
so 
\begin{align}
    \Qmag{2}\Qmag{3} \cos \theta_2 &= 
        \frac{1}{4m_a^2}
        \big[
            (t_2 - s_2 - m_a^2)(t_{3} - s_{3} - m_a^2) - 2m_a^2(t_2 + t_{3} - m_3^2)
        \big] \\
    \Qmag{1}\Qmag{3} \cos \theta_2 &= 
        \frac{1}{4m_a^2}
        \big[
            (t_2 - s_2 - m_a^2)(t_{3} - s_{3} - m_a^2) - 2m_a^2(t_2 + t_{3} - m_3^2)
        \big] \\
\end{align}